SEARZarith.sml
@@ -1,0 +1,441 @@
+val Fst_ex = prove_store("Fst_ex",
+e0
+(rpt strip_tac >> qexists_tac ‘Eval(p1(A,B),x)’ >> rw[])
+(form_goal
+ “!A B x:mem(A * B).?fstx. Eval(p1(A,B),x) = fstx”));
+
+ 
+val Snd_ex = prove_store("Snd_ex",
+e0
+(rpt strip_tac >> qexists_tac ‘Eval(p2(A,B),x)’ >> rw[])
+(form_goal
+ “!A B x:mem(A * B).?sndx. Eval(p2(A,B),x) = sndx”));
+
+val Fst_def = Fst_ex |> spec_all |> ex2fsym0 "Fst" ["x"]
+val Snd_def = Snd_ex |> spec_all |> ex2fsym0 "Snd" ["x"]
+
+val Pair_def' = Pair_def |> rewr_rule[Fst_def,Snd_def]
+
+val ZR_def = 
+fVar_Inst 
+[("P",([("mn",mem_sort $Cross N N),("m'n'",mem_sort $Cross N N)],
+ “Add(Fst(mn:mem(N * N)),Snd(m'n':mem(N * N))) = 
+ Add(Fst(m'n'),Snd(mn))”))] 
+(AX1 |> qspecl [‘N * N’,‘N * N’] |> uex_expand)
+|> ex2fsym0 "ZR" [] |> conjE1
+|> store_as "ZR_def";
+
+val ZR_Refl = prove_store("ZR_Refl",
+e0
+(rw[Refl_def,ZR_def])
+(form_goal
+ “Refl(ZR)”));
+
+val Pair_Fst_Snd = Pair_component |> rewr_rule[Fst_def,Snd_def] |> store_as "Pair_Fst_Snd";
+
+(*AQ how to let it realize 
+ !(a1 : mem(N * N))  (a2 : mem(N * N)).
+               Add(Fst(a1#), Snd(a2#)) = Add(Fst(a2#), Snd(a1#)) ==>
+               Add(Fst(a2#), Snd(a1#)) = Add(Fst(a1#), Snd(a2#))
+
+analoge of cases on ‘a1’
+*)
+
+
+local 
+val l =
+fVar_Inst 
+[("P",([("m",mem_sort N)],
+ “!n0 p. Add(m,Add(n0,p)) = Add(Add(m,n0),p)”))] 
+N_ind_P
+in
+val Add_assoc = prove_store("Add_assoc",
+e0
+(irule l >> rw[Add_O,Suc_def,Add_Suc,Add_Suc1,Add_O2] >>
+ rpt strip_tac >>arw[])
+(form_goal
+ “!m n0 p. Add(m,Add(n0,p)) = Add(Add(m,n0),p)”));
+end
+
+val Add_eq_eq = prove_store("Add_eq_eq",
+e0
+(rpt strip_tac >> 
+ qby_tac
+ ‘Sub(Add(m,a),a) = Sub(Add(n,a),a)’
+ >-- arw[] >>
+ fs[Add_Sub])
+(form_goal
+ “!m n a. Add(m,a) = Add(n,a) ==> m = n”));
+
+(*use add_sub*)
+val ZR_Trans = prove_store("ZR_Trans",
+e0
+(rw[Trans_def,ZR_def] >>
+ qsuff_tac
+ ‘!a1 b1 a2 b2 a3 b3.
+  Add(a1,b2) = Add(a2,b1) & Add(a2,b3) = Add(a3,b2) ==>
+  Add(a1,b3) = Add(a3,b1)’
+ >-- (rpt strip_tac >>
+     first_x_assum (qspecl_then [‘Fst(a1)’,‘Snd(a1)’,‘Fst(a2)’,‘Snd(a2)’,‘Fst(a3)’,‘Snd(a3)’] assume_tac) >>
+     first_x_assum irule >> arw[]) >>
+ rpt strip_tac >>
+ irule Add_eq_eq >> qexists_tac ‘b2’ >>
+ once_rw[GSYM Add_assoc] >>
+ qby_tac
+ ‘Add(b3,b2) = Add(b2,b3) & Add(b1,b2) = Add(b2,b1)’ 
+ >-- (strip_tac 
+     >-- qspecl_then [‘b2’,‘b3’] accept_tac Add_sym
+     >-- qspecl_then [‘b2’,‘b1’] accept_tac Add_sym) >>
+ arw[] >>
+ rw[Add_assoc] >> once_arw[] >> 
+ qpick_x_assum ‘Add(a2, b3) = Add(a3, b2)’
+ (assume_tac o GSYM) >> once_arw[] >>
+ rw[GSYM Add_assoc] >>
+ qspecl_then [‘b3’,‘b1’] assume_tac Add_sym >>
+ once_arw[] >> rw[])
+(form_goal
+ “Trans(ZR)”));
+
+val ZR_Sym = prove_store("ZR_Sym",
+e0
+(rw[ZR_def,Sym_def] >> rpt strip_tac >> flip_tac >>
+ arw[])
+(form_goal
+ “Sym(ZR)”));
+
+val ZR_ER = prove_store("ZR_ER",
+e0
+(rw[ER_def,ZR_Refl,ZR_Sym,ZR_Trans])
+(form_goal “ER(ZR)”));
+
+val toZ_def = 
+Thm_2_14 |> qspecl [‘N * N’,‘ZR’]
+         |> C mp ZR_ER
+         |> ex2fsym0 "Z" []
+         |> ex2fsym0 "toZ" []
+         |> store_as "toZ_def";
+
+val zj_ex = prove_store("zj_ex",
+e0
+(qexists_tac ‘Pair(O,O)’ >> rw[])
+(form_goal
+ “?zj.Pair(O,O) = zj”));
+
+val zj_def = zj_ex |> ex2fsym0 "0j" []
+                   |> store_as "zj_def";
+
+
+val oj_ex = prove_store("oj_ex",
+e0
+(qexists_tac ‘Pair(Suc(O),O)’ >> rw[])
+(form_goal
+ “?oj.Pair(Suc(O),O) = oj”));
+
+val oj_def = oj_ex |> ex2fsym0 "1j" []
+                   |> store_as "oj_def";
+
+val negj_def = 
+fVar_Inst 
+[("P",([("mn",mem_sort $Cross N N),("m'n'",mem_sort $Cross N N)],
+ “Fst(mn:mem(N * N)) = Snd(m'n') & Snd(mn) = Fst(m'n')”))] 
+(AX1 |> qspecl [‘N * N’,‘N * N’] |> uex_expand)
+|> ex2fsym0 "negj" [] |> conjE1
+|> store_as "negj_def";
+
+val negj_Fun = prove_store("negj_Fun",
+e0
+(rw[Fun_expand,negj_def] >> rpt strip_tac 
+ >-- (qexists_tac ‘Pair(Snd(a),Fst(a))’ >> 
+     rw[Pair_def']) >>
+ once_rw[Pair_component] >>
+ rw[Pair_eq_eq] >> rw[Fst_def,Snd_def] >>
+ pop_assum_list (map_every (assume_tac o GSYM)) >>
+ arw[])
+(form_goal
+ “isFun(negj)”));
+
+val Eval_negj = prove_store("Eval_negj",
+e0
+(rpt strip_tac >> assume_tac negj_Fun >>
+ drule $GSYM Eval_def >> flip_tac >>  
+ arw[] >> rw[negj_def] >>
+ rw[Pair_def'])
+(form_goal
+ “!m n. Eval(negj,Pair(m,n)) = Pair(n,m)”));
+
+
+val Negj_ex = prove_store("Negj_ex",
+e0
+(rpt strip_tac >> qexists_tac ‘Eval(negj,mn)’ >> rw[])
+(form_goal
+ “!mn.?nm.Eval(negj,mn) = nm”));
+
+val Negj_def = Negj_ex |> spec_all |> ex2fsym0 "Negj" ["mn"] |> store_as "Negj_def";
+
+val Negj_property = Eval_negj |> rewr_rule[Negj_def]
+                              |> store_as "Negj_property";
+
+
+
+
+
+val addj_def = 
+fVar_Inst 
+[("P",([("abcd",mem_sort (Cross (Cross N N) $Cross N N)),("acbd",mem_sort $Cross N N)],
+ “Fst(acbd) = Add(Fst(Fst(abcd:mem((N * N) * N * N))),Fst(Snd(abcd))) &
+  Snd(acbd) = Add(Snd(Fst(abcd)),Snd(Snd(abcd)))”))] 
+(AX1 |> qspecl [‘(N * N) * (N * N)’,‘N * N’] |> uex_expand)
+|> ex2fsym0 "addj" [] |> conjE1
+|> store_as "addj_def";
+
+val Fst_Snd_eq = Pair_Eval_eq |> rewr_rule[Fst_def,Snd_def] |> store_as "Fst_Snd_eq";
+
+val addj_Fun = prove_store("addj_Fun",
+e0
+(rw[Fun_expand,addj_def] >> rpt strip_tac 
+ >-- (qexists_tac ‘Pair(Add(Fst(Fst(a)), Fst(Snd(a))),Add(Snd(Fst(a)), Snd(Snd(a))))’ >> 
+     rw[Pair_def']) >>
+ irule Fst_Snd_eq >>
+ arw[])
+(form_goal
+ “isFun(addj)”));
+
+val Eval_addj = prove_store("Eval_addj",
+e0
+(rpt strip_tac >> assume_tac addj_Fun >>
+ drule $GSYM Eval_def >> flip_tac >>  
+ arw[] >> rw[addj_def] >>
+ rw[Pair_def'])
+(form_goal
+ “!a b c d. Eval(addj,Pair(Pair(a,b),Pair(c,d))) = Pair(Add(a,c),Add(b,d))”));
+
+
+val Addj_ex = prove_store("Addj_ex",
+e0
+(rpt strip_tac >> qexists_tac ‘Eval(addj,Pair(ab,cd))’ >> rw[])
+(form_goal
+ “!ab cd.?acbd.Eval(addj,Pair(ab,cd)) = acbd”));
+
+val Addj_def = Addj_ex |> spec_all |> ex2fsym0 "Addj" ["ab","cd"] |> store_as "Addj_def";
+
+val Addj_property = Eval_addj |> rewr_rule[Addj_def]
+                              |> store_as "Addj_property";
+
+val _ = new_pred "lej" [("ab",mem_sort (Cross N N)),
+                        ("cd",mem_sort (Cross N N))]
+
+val lej_def = store_ax("lej_def",
+“!ab cd.lej(ab,cd) <=> Le(Add(Fst(ab),Snd(cd)),Add(Snd(ab),Fst(cd)))”)
+
+
+val lej_property = prove_store("lej_property",
+e0
+(rw[lej_def,Pair_def'])
+(form_goal
+ “!a b c d.lej(Pair(a,b),Pair(c,d)) <=>
+ Le(Add(a,d),Add(b,c))”));
+
+
+val J1_i = prove_store("J1_i",
+e0
+(rw[Addj_property,GSYM Add_assoc,ZR_def])
+(form_goal
+ “!a b c d e f.
+ Holds(ZR,
+ Addj(Addj(Pair(a,b),Pair(c,d)),Pair(e,f)),
+ Addj(Pair(a,b),Addj(Pair(c,d),Pair(e,f))))”));
+
+val J1_ii = prove_store("J1_ii",
+e0
+(rw[GSYM zj_def,Addj_property,ZR_def,Add_O])
+(form_goal
+ “!a b.Holds(ZR,Addj(Pair(a,b),0j),Pair(a,b))”));
+
+val J1_iii = prove_store("J1_iii",
+e0
+(rw[Addj_property,GSYM zj_def,Negj_property,ZR_def,
+    Pair_def',Add_O,Add_O2] >>
+ rpt strip_tac >>
+ qspecl_then [‘b’,‘a’] assume_tac Add_sym >>
+ first_x_assum accept_tac)
+(form_goal
+ “!a b.Holds(ZR,Addj(Pair(a,b),Negj(Pair(a,b))),0j)”));
+
+val J1_iv = prove_store("J1_iv",
+e0
+(rw[Addj_property,ZR_def,Pair_def'] >>
+ rpt strip_tac >>
+ qspecl_then [‘c’,‘a’] assume_tac Add_sym >>
+ qspecl_then [‘b’,‘d’] assume_tac Add_sym >> 
+ arw[])
+(form_goal
+ “!a b c d.Holds(ZR,Addj(Pair(a,b),Pair(c,d)),
+                    Addj(Pair(c,d),Pair(a,b)))”));
+
+
+val J2_i = prove_store("J2_i",
+e0
+(rw[Addj_property,ZR_def,Pair_def'] >>
+ rpt strip_tac >>
+ rw[GSYM Add_assoc] >>
+ qspecl_then [‘d'’,‘b'’] assume_tac Add_sym >> arw[] >>
+ qspecl_then [‘c’,‘d'’,‘b'’] assume_tac Add_assoc >>
+ arw[] >>
+ rw[GSYM Add_assoc] >>
+ qspecl_then [‘Add(c',Add(d,b'))’,‘a’] 
+ assume_tac Add_sym >> arw[] >>
+ rw[GSYM Add_assoc] >>
+ qspecl_then [‘a’,‘b'’] assume_tac Add_sym >>
+ arw[] >>
+ qsspecl_then [‘Add(c', Add(b, d))’,‘a'’]
+ assume_tac Add_sym >> arw[] >>
+ rw[GSYM Add_assoc] >> 
+ qsuff_tac
+ ‘Add(d, Add(a', b)) = Add(b, Add(d, a'))’
+ >-- (strip_tac >> arw[]) >>
+ qspecl_then [‘Add(a',b)’,‘d’] assume_tac Add_sym >>
+ arw[] >> 
+ qspecl_then [‘a'’,‘d’] assume_tac Add_sym >> arw[] >>
+ rw[Add_assoc] >>
+ qspecl_then [‘a'’,‘b’] assume_tac Add_sym >> arw[])
+(form_goal
+ “!a b a' b' c d c' d'. Holds(ZR,Pair(a,b),Pair(a',b')) & Holds(ZR,Pair(c,d),Pair(c',d')) ==>
+ Holds(ZR,Addj(Pair(a,b),Pair(c,d)),Addj(Pair(a',b'),Pair(c',d')))”));
+
+val J2_ii = prove_store("J2_ii",
+e0
+(rw[ZR_def,Negj_property,Pair_def'] >> rpt strip_tac >>
+ qspecl_then [‘a'’,‘b’] assume_tac Add_sym >>
+ arw[] >> last_x_assum (assume_tac o GSYM) >> arw[] >>
+ qspecl_then [‘b'’,‘a’] accept_tac Add_sym)
+(form_goal
+ “!a b a' b'. Holds(ZR,Pair(a,b),Pair(a',b')) ==>
+  Holds(ZR,Negj(Pair(a,b)),Negj(Pair(a',b')))”));
+
+val rep_ex = prove_store("rep_ex",
+e0
+(strip_tac >> assume_tac toZ_def >>
+ fs[Surj_def] >> 
+ first_x_assum $ qspecl_then [‘z’] strip_assume_tac >>
+ qexists_tac ‘x’ >> arw[] >>
+ qexistsl_tac [‘Fst(x)’,‘Snd(x)’] >>
+ qsspecl_then [‘x’] accept_tac Pair_Fst_Snd)
+(form_goal
+ “!z. ?rz. Eval(toZ,rz) = z & ?a b. rz = Pair(a,b)”));
+
+val rep_def = rep_ex |> spec_all |> ex2fsym0 "rep" ["z"] |> gen_all |> store_as "rep_def";
+
+val Eval_rep = rep_def |> spec_all |> conjE1
+                       |> gen_all |> store_as "Eval_rep";
+
+val rcp_def = rep_def |> spec_all |> conjE2
+                      |> ex2fsym0 "rfst" ["z"]
+                      |> ex2fsym0 "rsnd" ["z"]
+                      |> gen_all
+                      |> store_as "rcp_def";
+
+val Eval_rcp = Eval_rep |> rewr_rule[rcp_def]
+                        |> store_as "Eval_rcp";
+
+val asz_ex = prove_store("asz_ex",
+e0
+(strip_tac >> qexists_tac ‘Eval(toZ,ab)’ >> rw[])
+(form_goal
+ “!ab.?z.Eval(toZ,ab) = z”));
+
+val asz_def = asz_ex |> spec_all |> ex2fsym0 "asz" ["ab"] |> gen_all |> store_as "asz_def";
+
+val rep_asz = Eval_rep |> rewr_rule[asz_def];
+
+val Z = mk_fun "Z" []
+(*
+val ADDz_def = 
+fVar_Inst 
+[("P",([("z1z2",mem_sort $Cross Z Z),("z",mem_sort Z)],
+ “Holds(ZR,Addj(
+  Pair(rfst(Fst(z1z2)),rsnd(Fst(z1z2))),
+  Pair(rfst(Snd(z1z2)),rsnd(Snd(z1z2)))),Pair(rfst(z),rsnd(z)))”))] 
+(AX1 |> qspecl [‘Z * Z’,‘Z’] |> uex_expand)
+|> ex2fsym0 "ADDz" [] |> conjE1
+
+*)
+
+val ADDz_def = 
+fVar_Inst 
+[("P",([("z1z2",mem_sort $Cross Z Z),("z",mem_sort Z)],
+ “Holds(ZR,Addj(rep(Fst(z1z2)),rep(Snd(z1z2))),rep(z))”))] 
+(AX1 |> qspecl [‘Z * Z’,‘Z’] |> uex_expand)
+|> ex2fsym0 "ADDz" [] |> conjE1
+
+
+val rep_asz_ZR = prove_store("rep_asz_ZR",
+e0
+(rw[GSYM asz_def] >>
+ assume_tac Eval_rep >>
+ rw[toZ_def] >> arw[])
+(form_goal
+ “!ab.Holds(ZR,ab,rep(asz(ab)))”));
+
+val corres_z_uex = prove_store("corres_z_uex",
+e0
+(strip_tac >> uex_tac >>
+ qexists_tac ‘asz(ab)’ >> rw[rep_asz_ZR] >>
+ rpt strip_tac >> 
+ fs[toZ_def,asz_def] >> rw[rep_asz])
+(form_goal
+ “!ab.?!z.Holds(ZR,ab,rep(z))”));
+
+val ADDz_Fun = prove_store("ADDz_Fun",
+e0
+(rw[Fun_expand,ADDz_def] >> rpt strip_tac >--
+ (qexists_tac ‘asz(Addj(rep(Fst(a)), rep(Snd(a))))’ >>
+ rw[rep_asz_ZR]) >>
+ qspecl_then [‘Addj(rep(Fst(a)), rep(Snd(a)))’]
+ assume_tac corres_z_uex  >>
+ pop_assum (assume_tac o uex_expand) >>
+ pop_assum strip_assume_tac >>
+ qsuff_tac
+ ‘b1 = z & b2 = z’
+ >-- (strip_tac >> arw[]) >> strip_tac >>
+ first_x_assum irule >> first_x_assum accept_tac)
+(form_goal
+ “isFun(ADDz)”));
+
+val Addz_ex = prove_store("Addz_ex",
+e0
+(rpt strip_tac >> 
+ qexists_tac ‘Eval(ADDz,Pair(z1,z2))’ >> rw[])
+(form_goal
+ “!z1 z2.?z12. Eval(ADDz,Pair(z1,z2)) = z12”));
+
+val Addz_def = Addz_ex |> spec_all 
+                       |> ex2fsym0 "Addz" ["z1","z2"] 
+                       |> gen_all
+                       |> store_as "Addz_def";
+
+val Addz_eqn = prove_store("Addz_eqn",
+e0
+(rpt strip_tac >>
+ rw[GSYM Addz_def] >>
+ assume_tac ADDz_Fun >>
+ drule $ GSYM Eval_def >> 
+ flip_tac >> arw[] >>
+ rw[ADDz_def,Pair_def',rep_asz_ZR])
+(form_goal
+ “!z1 z2.
+  Addz(z1,z2) = asz(Addj(rep(z1),rep(z2)))”));
+
+val ZR_samez = prove_store("ZR_samez",
+e0
+(rw[toZ_def,GSYM asz_def])
+(form_goal
+ “!ab cd. Holds(ZR,ab,cd) <=> asz(ab) = asz(cd)”));
+
+val Addz_sym = prove_store("Addz_sym",
+e0
+(rw[Addz_eqn] >> rw[GSYM ZR_samez] >> rpt strip_tac>>
+ once_rw[rcp_def] >> rw[J1_iv])
+(form_goal
+ “!z1 z2. Addz(z1,z2) = Addz(z2,z1)”));
+
+
